syncCoq.sh
@@ -1,6 +1,6 @@
 rsync -av --delete --exclude="asts" --exclude="**/#*" --exclude="**/*~" --exclude="**/.lia.cache" --exclude="**/.nia.cache" /home/abhishek/work/coq/blue/fm-workspace-snapshot3b/fm-workspace-12-16/fmdeps/monad/ monadproofs/
 git add monadproofs
-rsync -av --delete --exclude="**/#*" --exclude="**/*~" --exclude="**/.lia.cache" --exclude="**/.nia.cache" /home/abhishek/work/coq/blue/fm-workspace-snapshot3b/fm-workspace-12-16/fmdeps/evm-op-sem/ evm-op-sem/
+#rsync -av --delete --exclude="**/#*" --exclude="**/*~" --exclude="**/.lia.cache" --exclude="**/.nia.cache" /home/abhishek/work/coq/blue/fm-workspace-snapshot3b/fm-workspace-12-16/fmdeps/evm-op-sem/ evm-op-sem/
 git add monadproofs
-git add evm-op-sem
+#git add evm-op-sem
 
